src/extern/dotnet/Collections.cs
@@ -1,0 +1,37 @@
+using System;
+using System.IO;
+using ESDKClient;
+using STL;
+
+namespace Collections {
+    public partial class ExternByteProducer {
+        // TODO should be readonly, however we can't set in constructor due to
+        // weird extern-ness
+        private Stream stream;
+
+        public void SetInputStream(Stream stream) {
+            this.stream = stream;
+        }
+
+        // TODO ideally this shouldn't be used
+        // and instead we rely on a more efficient way
+        // to read from the input stream
+        public Result<byte> ExternNext() {
+            byte[] bytes = new byte[1];
+            stream.Read(bytes, 0, 1);
+            return Result<byte>.create_Success(bytes[0]);
+        }
+
+        // TODO Need to assume that input stream is seekable.
+        // If it is not, then we need to load everything into memory?
+        // For now, just assume
+        public bool ExternHasNext() {
+            return stream.Position != stream.Length;
+        }
+        
+        public int Length() {
+            // TODO cutting off int sizes
+            return (int)stream.Length;
+        }
+    }
+}
